last commit before I change DFA acceptance to be run-less and make runs a by-product. maybe.

automata.v
@@ -1,142 +1,213 @@
-Require Import ssreflect ssrbool eqtype fintype finfun seq fingraph ssrfun ssrnat.
+Require Import ssreflect ssrbool eqtype fintype finfun seq fingraph ssrfun ssrnat finset.
 
 Require Import misc.
 
 Set Implicit Arguments.
 
-(* Finite automata. *)
+(** Finite automata. ***)
 Section FA.
-(* input alphabet. *)
-Variable char: finType.
-(* Type of input sequences *)
-Definition word := seq char.
 
-(* Deterministic finite automata.
+(** The finite input alphabet. ***)
+Variable char: finType.
+
+(** Type of input sequences ***)
+Definition word := misc.word char.
+
+(** Deterministic finite automata.
    This is the only actual type of automata.
    NFAs will be translated on the fly (they
-   never exist as instances of some type). *)
+   never exist as instances of some type). ***)
 Section DFA.
 
-(* The (finite) type of states *)
+(** The finite type of states ***)
 Variable state: finType.
 
-(* The inductive type of deterministic finite automata *)
-Inductive dfa (s0: state) (fin: pred state) (step: state -> char -> state) : Type :=
-    | dfaI : dfa s0 fin step.
+(** The type of deterministic finite automata. ***)
+Record dfa : Type :=
+  dfaI {
+    dfa_s0: state;
+    dfa_fin: pred state;
+    dfa_step: state -> char -> state
+    }.
 
-
-(* Acceptance on DFAs *)
+(** Acceptance on DFAs **)
 Section Acceptance.
 
-(* Assume some automaton *)
-Variable s0_: state.
-Variable fin_: pred state.
-Variable step_: state -> char -> state.
-Variable A: dfa s0_ fin_ step_.
+(** Assume some automaton **)
+Variable A: dfa.
 
-(* This is a giant, steaming pile of hack.
-   (It forces all the following functions to
-   take an automaton as argument.) *)
-Definition A_s0 := [fun A: dfa s0_ fin_ step_ => s0_ ].
-Definition A_fin := [ fun A: dfa s0_ fin_ step_ => fin_ ].
-Definition A_step := [ fun A: dfa s0_ fin_ step_ => step_ ].
-Let s0 := A_s0 A.
-Let fin := A_fin A.
-Let step := A_step A.
-
-(* We define a run of w on the automaton A
+(** We define a run of w on the automaton A
    to be the list of states x_1 .. x_|w|
    traversed when following the edges labeled
-   w_1 .. w_|w| starting in x. *)
-Fixpoint run' (x: state) (w: word) : seq state :=
+   w_1 .. w_|w| starting in x. **)
+Fixpoint dfa_run' (x: state) (w: word) : seq state :=
 match w with
   | [::] => [::]
-  | a::w => (step x a) ::run' (step x a) w
+  | a::w => (dfa_step A x a) ::dfa_run' (dfa_step A x a) w
 end.
 
-(* A simplifying function for a "complete" run
-   (i.e. starting at s0). *)
-Definition run := [fun w => run' s0 w].
+(** A simplifying function for a "complete" run
+   (i.e. starting at s0). **)
+Definition dfa_run := [fun w => dfa_run' (dfa_s0 A) w].
 
-(* Acceptance of w in x is defined as
+(** Acceptance of w in x is defined as
    finality of the last state of a run of w on A
-   starting in x. *)
-Definition accept' := [ fun x w => fin (last x (run' x w) ) ].
+   starting in x. **)
+Definition dfa_accept' := [ fun x w => dfa_fin A (last x (dfa_run' x w) ) ].
 
-(* Acceptance of w on A starting in s0. *)
-Definition accept := [fun w => accept' s0 w].
+(** Acceptance of w on A starting in s0. **)
+Definition dfa_accept := [fun w => dfa_accept' (dfa_s0 A) w].
 
-(* A lemma that helps us avoid cumbersome unfolding of accept' *)
-Lemma accept'S x a w : accept' x (a::w) = accept' (step x a) w.
+(** A lemma that helps us avoid cumbersome unfolding of accept' **)
+Lemma dfa_accept'S x a w : dfa_accept' x (a::w) = dfa_accept' (dfa_step A x a) w.
 Proof. elim: w x a => [|b w IHw] x a //=. Qed.
-(* Same for run' *)
-Lemma run'S x a w : run' x (a::w) = (step x a) :: run' (step x a) w.
+(** Same for run' **)
+Lemma dfa_run'S x a w : dfa_run' x (a::w) = (dfa_step A x a) :: dfa_run' (dfa_step A x a) w.
 Proof. by []. Qed.
   
-(* The size of a run is the size of the input word. *)
-Lemma run_size x w : size (run' x w) = size w.
+(** The size of a run is the size of the input word. **)
+Lemma dfa_run_size x w : size (dfa_run' x w) = size w.
 Proof. elim: w x => [|a w IHw] x //=.
   by rewrite IHw.
 Qed.
 
-(* take lemma. *)
-Lemma run'_take x w n: take n (run' x w) = run' x (take n w).
+(** take lemma. **)
+Lemma dfa_run'_take x w n: take n (dfa_run' x w) = dfa_run' x (take n w).
 Proof. elim: w x n => [|a w IHw] x n //.
-rewrite run'S 2!take_cons. case: n => [|n] //.
-by rewrite IHw run'S.
+rewrite dfa_run'S 2!take_cons. case: n => [|n] //.
+by rewrite IHw dfa_run'S.
 Qed.
 
-(* rcons and cat lemmas. *)
-Lemma run'_cat x w1 w2 : run' x (w1 ++ w2) = run' x w1 ++ run' (last x (run' x w1)) w2.
+(** rcons and cat lemmas. **)
+Lemma dfa_run'_cat x w1 w2 : dfa_run' x (w1 ++ w2) = dfa_run' x w1 ++ dfa_run' (last x (dfa_run' x w1)) w2.
 Proof. elim: w1 w2 x => [|a w1 IHw1] w2 x //.
 simpl. by rewrite IHw1.
 Qed.
 
-Lemma run'_rcons x w a : run' x (rcons w a) = rcons (run' x w) (step (last x (run' x w)) a).
+Lemma dfa_run'_rcons x w a : dfa_run' x (rcons w a) = rcons (dfa_run' x w) (dfa_step A (last x (dfa_run' x w)) a).
 Proof. move: w a x. apply: last_ind => [|w b IHw] a x //.
-rewrite -3!cats1. rewrite 2!run'_cat. by [].
+rewrite -3!cats1. rewrite 2!dfa_run'_cat. by [].
 Qed.
 
   
 
-(* Predicate to distinguish between accepting
-   and non-accepting runs. *)
-Definition run_accepting := [fun x xs => fin (last x xs)].
+(** Predicate to distinguish between accepting
+   and non-accepting runs. **)
+Definition dfa_run_accepting := [fun x xs => dfa_fin (last x xs)].
 
-Definition run_accepts x xs w := xs = run' x w.
+Definition dfa_run_accepts x xs w := xs == dfa_run' x w.
 
 End Acceptance.
 
-
 End DFA.
 
-(* Non-deterministic automata. These exist only
-   implicitly as non-functional transitions. *)
+
+
+(** Non-deterministic automata. **)
 Section NFA.
 
-(* Usual stuff. *)
+(** The finite type of states ***)
 Variable state: finType.
-Variable s0: state.
-Variable fin: pred state.
+  
+(** The type of non-deterministic finite automata. ***)
+Record nfa : Type :=
+  nfaI {
+    nfa_s0: state;
+    nfa_fin: pred state;
+    nfa_step: state -> char -> pred state
+    }.
 
-(* Non-functional transitions. *)
-Variable step_rel: state -> char -> pred state.
+(** Acceptance on non-deterministic automata. **)
+Section Acceptance.
 
-(* Type of states after powerset construction. *)
-Definition state_det := [ finType of {ffun state -> bool_eqType} ].
+Variable A: nfa.
 
-(* Finality predicate after powerset construction. *)
-Definition fin_det := [ fun q': state_det => existsb q:state, q' q && fin q ].
-Definition s0_det : state_det := [ ffun q:state => q==s0 ].
+(** Non-deterministic acceptance. **)
+Fixpoint nfa_accept' (x: state) w :=
+match w with
+  | [::] => nfa_fin A x
+  | a::w => existsb y, (nfa_step A x a y) && nfa_accept' y w
+end.
 
-(* Functional step after powerset construction. *)
-Definition step_det := [ fun (x': state_det) (a: char) => 
-[ ffun x => existsb y: state, x' y && step_rel y a x ] ].
+(** We define labeled paths over the non-deterministic step relation **)
+Fixpoint nfa_lpath x (xs : seq state) (w: word) {struct xs} :=
+match xs,w with
+  | y :: xs', a::w' => nfa_step A x a y && nfa_lpath y xs' w'
+  | [::]    , [::]  => true
+  | _       , _     => false
+end.
 
-(* Conversion from a non-functional transitions to a DFA. *)
-Definition to_dfa := dfaI state_det s0_det fin_det step_det.
+(** We proof that there is a path labeled with w induced
+   by nfa_accept' starting at x and ending in an accepting
+   state. **)
+Lemma nfa_accept_lpath x w: nfa_accept' x w -> exists xs, nfa_lpath x xs w /\ nfa_fin A (last x xs).
+Proof. elim: w x => [|a w IHw] x.
+  by exists [::].
+move => /existsP [] y /andP [] H0 /IHw [xs [H1 H2]].
+exists (y::xs) => /=.
+by rewrite H0 H1 H2.
+Qed.
+
+(** We proof that the existence of a path labeled with w
+   implies the acceptance of w. **)
+Lemma nfa_lpath_accept x xs w: nfa_lpath x xs w /\ nfa_fin A (last x xs) -> nfa_accept' x w.
+Proof. elim: w x xs => [|a w IHw] x xs.
+  (* We destruct the path to ensure that it is empty. *)
+  case: xs => [|y xs].
+    move/andP => []. by [].
+  (* Non-empty paths can not be not be produced by empty words. *)
+  by move/andP.
+case: xs => [|y xs].
+  (* Empty paths can not accept non-empty words. *)
+  by move/andP.
+simpl. move => [] /andP [] H0 H1 H2.
+apply/existsP. exists y.
+rewrite H0 andTb. apply: IHw.
+split; eassumption.
+Qed.
+
+End Acceptance.
 
 End NFA.
+
+(** We define the powerset construction to obtain
+   a deterministic automaton from a non-deterministic one. **) 
+Section PowersetConstruction.
+
+Variable state: finType.
+Variable A: nfa state.
+
+(** The new automaton's states are sets of the given
+   automatons' states. **)
+Definition powerset_state : finType := [finType of {set state}].
+
+
+Definition nfa_to_dfa :=
+  dfaI
+    powerset_state
+    (set1 (nfa_s0 A))
+    [ pred X: powerset_state | existsb x: state, (x \in X) && nfa_fin A x]
+    [fun X a => cover [set finset (nfa_step A x a) | x <- X] ]
+.
+
+(** We prove that nfa_to_dfa builds an automaton which
+   accepts exactly the language of the given automaton.
+   We first prove that, for every state x, the new automaton
+   accepts the same language when starting in a set containing x. **)
+Lemma nfa_to_dfa_correct (x: state) w (X: powerset_state): x \in X -> (nfa_accept' A x w <-> dfa_accept' nfa_to_dfa X w).
+Proof. move => H0. split.
+  (* "->" *)
+  elim: w x H0 => [|a w IHw] x H0.
+    (* [::] *)
+    move => /= H1. apply/existsP. exists x.
+    by rewrite H0 H1.
+  (* a::w *)
+  move/nfa_accept_lpath => [] y [] H1 H2.
+  move/existsP => [] y /andP [] H1 H2.
+  
+
+
+End PowersetConstruction.
 
 End FA.
 
@@ -144,7 +215,7 @@ Hint Unfold A_step.
 Hint Unfold A_s0.
 Hint Unfold A_fin.
 
-(* Operations on up to two automata with the same alphabet *)
+(** Operations on up to two automata with the same alphabet **)
 Section Operators.
 Variable char: finType.
 Variable state1 state2: finType.
@@ -159,16 +230,16 @@ Variable A1: dfa char state1 s01 fin1 step1.
 Variable A2: dfa char state2 s02 fin2 step2.
 
 
-(* Complement automaton *)
+(** Complement automaton **)
 Section Complement.
   
-(* The only change needed is to negate the finality predicate. *)
+(** The only change needed is to negate the finality predicate. **)
 Definition fin_not := [ fun q1 => ~~ fin1 q1 ].
-(* We construct the resulting automaton. *)
+(** We construct the resulting automaton. **)
 Definition Aut_not := dfaI char state1 s01 fin_not step1.
 
-(* We proof that the complement automaton accepts exactly
-   the words not accepted by the original automaton. *)
+(** We proof that the complement automaton accepts exactly
+   the words not accepted by the original automaton. **)
 Lemma Aut_not_correct w q: accept' A1 q w = ~~ accept' Aut_not q w.
 Proof.
   by apply/idP/negPn.
@@ -177,11 +248,11 @@ Qed.
 End Complement.
 
 
-(* Cross product of the two state sets *)
+(** Cross product of the two state sets **)
 Definition state_prod := prod_finType state1 state2.
 
 
-(* Disjunction automaton *)
+(** Disjunction automaton **)
 Section Disjunction.
 
 Definition step_or (q: state_prod) a := let (q1, q2) := q in (step1 q1 a, step2 q2 a).
@@ -189,7 +260,7 @@ Definition Aut_or := dfaI char state_prod (s01, s02)
 (fun q => let (q1,q2) := q in fin1 q1 || fin2 q2)
 step_or.
 
-(* Correctness w.r.t. any state. *)
+(** Correctness w.r.t. any state. **)
 Lemma Aut_or_correct' w q1 q2 : accept' A1 q1 w || accept' A2 q2 w = accept' Aut_or (q1, q2) w.
 Proof. elim: w q1 q2 => [|a w IHw].
   rewrite/accept => //.
@@ -197,14 +268,14 @@ rewrite/accept => /=. move => q1 q2.
 by exact: IHw.
 Qed.
 
-(* Language correctness. *)
+(** Language correctness. **)
 Lemma Aut_or_correct w: accept A1 w || accept A2 w = accept Aut_or w.
 Proof. exact: Aut_or_correct'. Qed.
 
 End Disjunction.
   
 
-(* Conjunction *) 
+(** Conjunction **) 
 Section Conjunction.
   
 Definition step_and (q: state_prod) a := let (q1, q2) := q in (step1 q1 a, step2 q2 a).
@@ -212,7 +283,7 @@ Definition Aut_and := dfaI char state_prod (s01, s02)
 (fun q => let (q1,q2) := q in fin1 q1 && fin2 q2)
 step_or.
 
-(* Correctness w.r.t. any state. *)
+(** Correctness w.r.t. any state. **)
 Lemma Aut_and_correct' w q1 q2 : accept' A1 q1 w && accept' A2 q2 w = accept' Aut_and (q1, q2) w.
 Proof. elim: w q1 q2 => [|a w IHw].
   rewrite/accept => //.
@@ -220,68 +291,68 @@ rewrite/accept => /=. move => q1 q2.
 by exact: IHw.
 Qed.
 
-(* Language correctness. *)
+(** Language correctness. **)
 Lemma Aut_and_correct w: accept A1 w && accept A2 w = accept Aut_and w.
 Proof. exact: Aut_and_correct'. Qed.
 
 End Conjunction.
 
 
-(* Star automaton. *)
+(** Star automaton. **)
 Section Star.
   
-(* We need to add a new state. *)
+(** We need to add a new state. **)
 Definition state_star' := option_finType state1.
 Definition s0_star' : state_star' := None.
-(* We only accept the empty state. *)
+(** We only accept the empty state. **)
 Definition fin_star' := [ pred x | x == s0_star' ].
-(* The type of states in the star automaton. *)
+(** The type of states in the star automaton. **)
 Definition state_star := state_det state_star'.
-(* We construct a non-functional relation which is 
+(** We construct a non-functional relation which is 
    the new transitions of the star automaton.
    Whenever we enter a former final state, we
    also enter the new starting state, thereby
-   ensuring acceptance. *)
+   ensuring acceptance. **)
 Definition step_rel_star : state_star' -> char -> pred state_star' :=
   (fun x1 a =>
     match x1 with
-      (* any old state *)
+      (** any old state **)
       | Some x1 => [ pred x2 |
                        (x2 == Some (step1 x1 a))
                     || (fin1 (step1 x1 a) && (x2 == s0_star'))
                    ]
-      (* the new state s0_sta *)
+      (** the new state s0_sta **)
       | s0_star' => [ pred x2 | x2 == Some (step1 s01 a) ]
     end
   ).
-(* We construct the star automaton. *)
-(* Definition Aut_star := to_dfa char state1 s01 fin_star' step_rel_star. *)
+(** We construct the star automaton. **)
+(** Definition Aut_star := to_dfa char state1 s01 fin_star' step_rel_star. **)
 Definition step_star := step_det char step_rel_star.
 Definition s0_star := s0_det state_star' s0_star'.
 Definition fin_star := fin_det state_star' fin_star'.
 Definition Aut_star := dfaI char (state_det state_star') s0_star fin_star step_star.
 
-(* Starting state correctness. *)
+(** Starting state correctness. **)
 Lemma Aut_star_s0 : s0_star s0_star'. by rewrite /s0_star /s0_det ffunE eq_refl. Qed.
 
-(* step_star_rel invariant. *)
+(** step_star_rel invariant. **)
 Lemma Aut_star_step_rel (X: state_star) a: fin_star (step_star X a) -> (step_star X a) s0_star'.
 Proof. simpl. move/existsP => [] x. by rewrite andbC => /andP [] /eqP ->. Qed.
   
-(* We proof that the empty word is contained in the
-   language of the star automaton. *)
+(** We proof that the empty word is contained in the
+   language of the star automaton. **)
 Lemma Aut_star_correct0 : accept Aut_star [::].
 Proof. rewrite/accept/accept'/fin_star => /=. apply/existsP. exists s0_star'.
 by rewrite /s0_det ffunE eq_refl. Qed.
 
-(* We proof that all non-empty words accepted by the
+(** We proof that all non-empty words accepted by the
    original automaton are also accepted by the star
    automaton.
    Translating x to [pred x' | x'==x] gives us an
    induction hypothesis which is too weak to prove
    the statement. Therefore, we allow the star automaton
    to start from any set of states containing x.
-   *)
+   **)
 Lemma Aut_star_correctS (X: state_star) a w x :
   X (Some x) -> accept' A1 x (a::w) -> accept' Aut_star X (a::w).
 Proof. elim: w a X x => [| b w IHw ] a X x H0.
@@ -292,20 +363,20 @@ rewrite accept'S. apply: IHw. rewrite ffunE. apply/existsP. exists (Some x).
 by rewrite H0 andTb /step_rel_star /= eq_refl.
 Qed.
 
-(* We show that every accepting run of the
-   star automaton ends in a state Y s.t. Y s0_star'. *)
+(** We show that every accepting run of the
+   star automaton ends in a state Y s.t. Y s0_star'. **)
 Lemma Aut_star_end X w: accept' Aut_star X w -> last X (run' Aut_star X w) s0_star'.
 Proof. elim: w X => [|a w IHw] X.
   by move => /= /existsP [] q /andP [] H0 /eqP <-.
 rewrite accept'S. by apply: IHw.
 Qed.
 
-(* We define the notion of a shortest, non-empty, accepting prefix *)
+(** We define the notion of a shortest, non-empty, accepting prefix **)
 Definition Aut_star_prefix (X: state_star) (w: word char) (n: nat) : bool :=
       (n > 0) && (n <= size w) && (accept' Aut_star X (take n w)) &&
   forallb n': ordinal n, (n' > 0) ==> ~~ accept' Aut_star X (take n' w).
  
-(* We proof that there are no shorter prefixes than the shortest prefix. *)
+(** We proof that there are no shorter prefixes than the shortest prefix. **)
 Definition Auf_star_prefix_shortest (X: state_star) (w: word char) (n: nat) :
   Aut_star_prefix X w n -> forallb n' : 'I_n, ~~ Aut_star_prefix X w n'.
 Proof. move: w X. apply: last_ind => [| w b IHw ] X.
@@ -319,7 +390,7 @@ move/neq0_lt0n => H4. apply/orP. right.
 move: (H3 m) => /implyP. move => H5. apply: H5. by [].
 Defined.
 
-(* This, too. *)
+(** This, too. **)
 Lemma word_expand (w: word char) : 0 < (size w) -> exists a, w = rcons (take (size w).-1 w) a.
 Proof. move: w. apply: last_ind => [| w a IHw].
   by [].
@@ -329,8 +400,8 @@ rewrite -cats1 takel_cat.
 by rewrite size_cat addn1.
 Qed.
 
-(* We proof that Aut_star_prefix is "transitive" regarding
-   additional suffixes. *)
+(** We proof that Aut_star_prefix is "transitive" regarding
+   additional suffixes. **)
 Lemma Aut_star_prefix_trans X w k m:
 k >= m -> Aut_star_prefix X (take k w) m -> Aut_star_prefix X w m.
 Proof. move: w m k. apply: last_ind => [|w b IHw] m k.
@@ -339,7 +410,7 @@ move => H0.
 case_eq (k < size (rcons w b)) => H1.
   rewrite -cats1 takel_cat.
     move/andP => [] /andP [] /andP [] H2 H3 H4 /forallP H5.
-    (* we'll need this a few times: *)
+    (** we'll need this a few times: **)
     have: m <= size w.
       apply: leq_trans.
         by apply H3.
@@ -375,8 +446,8 @@ move: (negbT H1). rewrite -leqNgt => H2.
 by rewrite take_oversize.
 Qed.
 
-(* We proof that there are no accepted prefixes < n if there is
-   no shortest, non-empty, accepting prefix < n *)
+(** We proof that there are no accepted prefixes < n if there is
+   no shortest, non-empty, accepting prefix < n **)
 Lemma Aut_star_prefix_none X w a n:
   0 < n ->
   (forallb m : 'I_(S n), (0 < m) ==> ~~ Aut_star_prefix X (rcons w a) m) -> ~~ accept' Aut_star X (take n (rcons w a)).
@@ -421,14 +492,14 @@ move: (H4 H7). rewrite 3!negb_and. rewrite H7. rewrite orFb.
      
 Admitted.
 
-(* We proof that there is a shortest, non-empty, accepting prefix
-   for every non-empty word accept by the star automaton. *)
+(** We proof that there is a shortest, non-empty, accepting prefix
+   for every non-empty word accept by the star automaton. **)
 Lemma Aut_star_shortest_prefix (X: state_star) (a: char) w:
   accept' Aut_star X (rcons w a) ->
   exists n,
     Aut_star_prefix X (rcons w a) n.
 Proof.
-(* We use size_induction to get a helpful IH. *)
+(** We use size_induction to get a helpful IH. **)
 move: w a X. apply: (size_induction size) => w IHw a X.
 case_eq (size w) => [|s] Hs.
   rewrite (size0nil Hs).
@@ -437,20 +508,20 @@ case_eq (size w) => [|s] Hs.
     rewrite andTb. by exact: H0. 
   apply/forallP => x. apply/implyP. move: (ltn_ord x).
   rewrite leq_eqVlt => /andP [] /eqP H1.
-  (* this is a very convoluted way of proving that x=0. *)
+  (** this is a very convoluted way of proving that x=0. **)
   case_eq (nat_of_ord x) => [|x'].
     by [].
   move/(f_equal S). rewrite H1. move/(f_equal predn). by [].
 
-(* We use word_expand to get separate prefix and the 1-suffix *)
+(** We use word_expand to get separate prefix and the 1-suffix **)
 have: 0 < size w.
   by rewrite Hs.
 move/word_expand => [] b Hw. rewrite Hw.
 move Ew: (take (size w).-1 w) => w'.
 move => H0.
-(* See if there already is a prefix: *)
+(** See if there already is a prefix: **)
 case_eq (existsb m : 'I_ (size (rcons (rcons w' b) a)), Aut_star_prefix X (rcons w' b) m).
-(* prefix. *)
+(** prefix. **)
   move/existsP => [] m /andP [] /andP [] /andP [] H1 H2 H3 /forallP H4.
   pose n:=nat_of_ord m.
   exists n. apply/andP. split.
@@ -464,7 +535,7 @@ case_eq (existsb m : 'I_ (size (rcons (rcons w' b) a)), Aut_star_prefix X (rcons
   rewrite -cats1 takel_cat. move: H5. apply/implyP. by exact: H4.
   apply: leq_trans. apply ltnW. apply ltn_ord. by [].
 
-(* no prefix. *)
+(** no prefix. **)
 
 move/negbT. rewrite negb_exists => /forallP H1. exists (size (rcons (rcons w' b) a)).
 apply/andP. split.
@@ -473,7 +544,7 @@ apply/andP. split.
   rewrite take_size. by exact: H0.
 apply/forallP => n'. apply/implyP => H2.
 move: (H1 n').
-(* We'll need this a few times. *)
+(** We'll need this a few times. **)
 have: (n' <= size (rcons w' b)).
     rewrite -{1}ltnS -(size_rcons (rcons w' b ) a).
     exact: (ltn_ord n').
@@ -490,8 +561,8 @@ rewrite negb_and H2 => /orP [].
 rewrite negb_forall.
 rewrite negb_forall_in.
 move/existsP => [] m.
-(* take m w' would be the shortest, non-empty, accepting prefix
-   but there is no such prefix. *)
+(** take m w' would be the shortest, non-empty, accepting prefix
+   but there is no such prefix. **)
 move/andP => [] H4 /negbNE H5.
 Admitted.
 
@@ -527,7 +598,7 @@ Admitted.
   
 End Star.
 
-(* Concatenation *)
+(** Concatenation **)
 Section Concatenation.
   
 Definition state_sum := sum_finType state1 state2.
@@ -559,12 +630,12 @@ match x with
 end ].
 Definition Aut_conc := to_dfa char state_sum (s0_conc) fin_conc step_conc. 
 
-(* We define a relation (an order) on states. *)
+(** We define a relation (an order) on states. **)
 Definition state_conc_leq (q1' q2': state_conc) := forall q, q1' q -> q2' q.
 
 Notation "q1' ===> q2'" := (state_conc_leq q1' q2') (at level 70).
 
-(* We proof a few interesting properties of this relation. *)
+(** We proof a few interesting properties of this relation. **)
 Lemma q_conc_leq_trans (q1' q2' q3': state_conc) : q1' ===> q2' -> q2' ===> q3' -> q1' ===> q3'.
 Proof. rewrite/state_conc_leq. move => H0 H1 q. by move/H0/H1. Qed.
 
@@ -585,9 +656,9 @@ move => q1' q2'. move/(@q_conc_leq_d_trans _ _ a). simpl.
 by apply: IHw.
 Qed.
 
-(* We proof that the concatenation automaton accepts
+(** We proof that the concatenation automaton accepts
    all words of the first automaton if the second automaton
-   accepts the empty word. *)
+   accepts the empty word. **)
 Lemma Aut_conc_correct1' q1 w1: 
 accept' A1 q1 w1 && accept A2 [::] 
 -> accept' Aut_conc (finfun (fun q=> q == state1_conc q1)) w1.
@@ -611,9 +682,9 @@ rewrite/step_conc => /=. by apply/eq_refl.
 Qed.
 
 
-(* We proof that the concatenation automaton accepts
+(** We proof that the concatenation automaton accepts
    all words accepted by the second automaton when if
-   they both start in the same state. *)
+   they both start in the same state. **)
 Lemma Aut_conc_correct2' x2 w2: 
 accept' A2 x2 w2
 -> accept' Aut_conc (finfun (fun x=> x == state2_conc x2)) w2.
@@ -627,8 +698,8 @@ apply/existsP. exists (state2_conc x2). apply/andP. split.
 by rewrite/step_conc => /=.
 Qed.
 
-(* We proof that final states of the first automaton have at
-   least all transitions of s02 in the concatenation automaton. *)
+(** We proof that final states of the first automaton have at
+   least all transitions of s02 in the concatenation automaton. **)
 Lemma Aut_conc_end1 x1 a:
 fin1 x1 ->
 step_det char step_conc [ffun x => x == state2_conc s02] a ===> step_det char step_conc [ffun x => x == state1_conc x1] a.
@@ -640,9 +711,9 @@ rewrite eq_sym ffunE => /eqP ->. apply/existsP. exists (state1_conc x1).
 rewrite ffunE eq_refl andTb. by rewrite H0 eq_refl.
 Qed.
 
-(* We proof that all words accepted by s02 are also accepted
+(** We proof that all words accepted by s02 are also accepted
    by final states of the first automaton in the concatenation
-   automaton. *)
+   automaton. **)
 Lemma Aut_conc_correct3' x1 w2:
 fin1 x1 ->
 accept' Aut_conc [ffun x => x == state2_conc s02] w2 ->
@@ -653,9 +724,9 @@ Proof. elim: w2 x1 => [|a w2 IHw2] x1 H0 /=.
 apply: Aut_conc_expand1. apply: Aut_conc_end1. exact: H0.
 Qed.
 
-(* We proof that the concatenation automaton accepts
+(** We proof that the concatenation automaton accepts
    all words that are made up of a prefix accepted by the first automaton
-   and a suffix accepted by the second automaton. *)
+   and a suffix accepted by the second automaton. **)
 Lemma Aut_conc_correct1 x1 w1 w2: (accept' A1 x1 w1 && accept A2 w2) ->
   accept' Aut_conc [ffun x => x == state1_conc x1] (w1 ++ w2).
 Proof. elim: w1 w2 x1 => [|a w1 IHw1] w2 x1.
@@ -666,9 +737,9 @@ rewrite /step_det /step_conc ffunE => /eqP -> /=. rewrite ffunE. apply/existsP.
 exists (state1_conc x1). by rewrite ffunE eq_refl andTb eq_refl.
 Qed.
 
-(* We proof that the concatenation automaton only accepts
+(** We proof that the concatenation automaton only accepts
    words that can be expressed as a prefix accepted by the first automaton
-   and a suffix accepted by the second automaton. *)
+   and a suffix accepted by the second automaton. **)
 Lemma Aut_conc_correct2 w: 
 accept' Aut_conc [ffun x => x == state1_conc s01] w -> 
 exists w1, exists w2, w = w1 ++ w2 /\ accept A1 w1 && accept A2 w2.
